fix range_map axiom.

crates/move-prover-boogie-backend/src/boogie_backend/prelude/native.bpl
@@ -988,8 +988,8 @@ function $RangeMapQuantifierHelper_{{FN}}({{QP}}): Vec ({{RT}});
 axiom (forall {{QP}}:: {$RangeMapQuantifierHelper_{{FN}}({{QA}})}
 (
     var res := $RangeMapQuantifierHelper_{{FN}}({{QA}});
-        LenVec(res) == end - start &&
-        (forall i: int :: start <= i && i < end ==> ReadVec(res, i - start) == {{FN}}({{EAB}}i{{EAA}}))
+        LenVec(res) == (if start <= end then end - start else 0) &&
+        (forall i: int :: InRangeVec(res, i) ==> ReadVec(res, i) == {{FN}}({{EAB}}(i + start){{EAA}}))
     )
 );
 {%- endif %}
